LeanMove/Tests/Parsing/AllParseTests.lean
@@ -41,6 +41,7 @@ import LeanMove.Tests.Parsing.Test_enum_borrow_owned
 import LeanMove.Tests.Parsing.Test_comparison_ops
 import LeanMove.Tests.Parsing.Test_casts
 import LeanMove.Tests.Parsing.Test_bitwise
+import LeanMove.Tests.Parsing.Test_arith_ops
 
 /-! ## All Parse Tests
 
